Mutual recursion, sort of

theories/iris/logrel/iris_rwasm_logrel.v
@@ -10,6 +10,7 @@ From Wasm.iris.helpers Require Export iris_properties.
 From Wasm.iris.language Require Export iris_atomicity.
 From Wasm.iris.rules Require Export iris_rules.
 From Wasm Require rwasm_datatypes.
+
 Import uPred.
 
 Section logrel.
@@ -29,24 +30,22 @@ Section logrel.
   (* ---------------------------------- VALUE RELATION ------------------------------------- *)
   (* --------------------------------------------------------------------------------------- *)
 
-  (* TODO: Make this actually mutually recursive. *)
-  Definition interp_value_recursive (τs : rwasm_datatypes.result_type) : WsR := λne ws, ⌜false⌝%I.
-
-  Definition interp_heap_value_struct (fs : list (rwasm_datatypes.value_type * rwasm_datatypes.size)) : HR :=
+  Definition interp_heap_value_struct
+    (fs : list (rwasm_datatypes.value_type * rwasm_datatypes.size))
+    (iv : rwasm_datatypes.value_type -> WsR)
+  : HR :=
     λne (bs : leibnizO bytes), (
       ∃ (bss : list bytes), ∃ (bs' : bytes),
         ⌜bs = flatten bss ++ bs'⌝ ∗
         [∗ list] f;bs'' ∈ fs;bss,
           let '(τ, sz) := f in
           ⌜rwasm_datatypes.eval_size sz = Some (length bs'')⌝ ∧
-          ∃ ws,
-            ⌜rwasm_datatypes.read τ bs'' = ws⌝ ∗
-            interp_value_recursive [τ] (Stack ws)
+          ∃ ws, ⌜rwasm_datatypes.read τ bs'' = ws⌝ ∗ iv τ (Stack ws)
     )%I.
-  
-  Definition interp_heap_value (Ψ : rwasm_datatypes.heap_type) : HR :=
+
+  Definition interp_heap_value (Ψ : rwasm_datatypes.heap_type) (iv : rwasm_datatypes.value_type -> WsR) : HR :=
     match Ψ with
-    | rwasm_datatypes.StructType fields => interp_heap_value_struct fields
+    | rwasm_datatypes.StructType fields => interp_heap_value_struct fields iv
     end.
 
   Definition interp_pre_value_unit : WsR := λne ws, ⌜∃ z, stack_values ws = [VAL_int32 z]⌝%I.
@@ -69,7 +68,12 @@ Section logrel.
     λne ws, ⌜false⌝%I.
 
   (* TODO: Check r/rw privilege. *)
-  Definition interp_pre_value_ref (π : rwasm_datatypes.cap) (sz : rwasm_datatypes.size) (ψ : rwasm_datatypes.heap_type) : WsR :=
+  Definition interp_pre_value_ref
+    (π : rwasm_datatypes.cap)
+    (sz : rwasm_datatypes.size)
+    (ψ : rwasm_datatypes.heap_type)
+    (iv : rwasm_datatypes.value_type -> WsR)
+  : WsR :=
     λne ws, (
       ∃ bs, ∃ z,
       ⌜stack_values ws = [VAL_int32 z]⌝ ∗
@@ -77,26 +81,38 @@ Section logrel.
       ([∗ list] k ↦ b ∈ bs,
         let n := Z.to_N (Wasm_int.Int32.unsigned z) in
         (N.add n (N.of_nat k)) ↦[wm][ N.of_nat 0 ] b) ∗
-      interp_heap_value ψ bs
+      interp_heap_value ψ iv bs
     )%I.
 
-  Definition interp_pre_value (p : rwasm_datatypes.pre_type) : WsR :=
+  Definition interp_pre_value (p : rwasm_datatypes.pre_type) (iv : rwasm_datatypes.value_type -> WsR) : WsR :=
     match p with
     | rwasm_datatypes.Num np => interp_pre_value_num np
     | rwasm_datatypes.Unit => interp_pre_value_unit
     | rwasm_datatypes.CoderefT Χ => interp_pre_value_coderef Χ
     | rwasm_datatypes.ExLoc τ' => interp_pre_value_exloc τ'
-    | rwasm_datatypes.RefT π sz ψ => interp_pre_value_ref π sz ψ
+    | rwasm_datatypes.RefT π sz ψ => interp_pre_value_ref π sz ψ iv
     end.
 
   (* TODO: Check qualifier. *)
-  Definition interp_value (τ : rwasm_datatypes.value_type) : WsR :=
-    match τ with
-    | rwasm_datatypes.QualT p q => interp_pre_value p
-    end.
+  Definition interp_value_0 (iv : leibnizO rwasm_datatypes.value_type -n> WsR) : (leibnizO rwasm_datatypes.value_type -n> WsR) :=
+    λne (τ : leibnizO rwasm_datatypes.value_type),
+      match τ with
+      | rwasm_datatypes.QualT p q => interp_pre_value p iv
+      end.
 
   (* TODO *)
+  Global Instance interp_value_contractive : Contractive interp_value_0.
+  Proof.
+    solve_proper_prepare.
+  Admitted.
+
+  Definition interp_value : (leibnizO rwasm_datatypes.value_type -n> WsR) := fixpoint interp_value_0.
+
+  (* TODO: Read the sequence of concrete values. *)
   Definition interp_val (τs : rwasm_datatypes.result_type) : VR :=
-    λne v, ⌜false⌝%I.
+    λne (v : leibnizO val), (
+      ⌜v = trapV⌝ ∨
+      ∃ ws, ⌜v = immV ws⌝ ∗ [∗ list] τ;w ∈ τs;ws, interp_value τ (Stack [w])
+    )%I.
 
 End logrel.
